Gcd now evaluates correctly in L1, L2 and L3.

theories/L1g/wndEval.v
@@ -39,8 +39,8 @@ Inductive wndEval : Term -> Term -> Prop :=
      (* Case argument must be in Canonical form *)
      (* n is the number of parameters of the datatype *)
 | sCase: forall (ml:inductive * nat * list nat) (ty s mch:Term)
-                 (args brs ts:Terms) (n:nat),
-            canonicalP mch = Some (n, args) ->
+                 (args brs ts:Terms) (n arty:nat),
+            canonicalP mch = Some (n, args, arty) ->
             tskipn (snd (fst ml)) args = Some ts ->
             whCaseStep n ts brs = Some s ->
             wndEval (TCase ml ty mch brs) s
