theories/L2_typeStripped/compile.v
@@ -1,6 +1,6 @@
 (****)
 Add LoadPath "../common" as Common.
-Add LoadPath "../L1_5_box" as L1_5.
+Add LoadPath "../L1g" as L1g.
 (****)
 
 Require Import Coq.Lists.List.
@@ -8,25 +8,26 @@ Require Import Coq.Strings.String.
 Require Import Coq.Arith.Compare_dec.
 Require Import Coq.Arith.Peano_dec.
 Require Import Common.Common.
-Require Import L1_5.compile.
+Require Import L1g.compile.
+Require Import L1g.term.
 
 Local Open Scope string_scope.
 Local Open Scope bool.
 Local Open Scope list.
 Set Implicit Arguments.
 
-Definition L1_5Term := L1_5.compile.Term.
-Definition L1_5Terms := L1_5.compile.Terms.
-Definition L1_5Defs := L1_5.compile.Defs.
-Definition L1_5Pgm := Program L1_5Term.
-Definition L1_5EC := envClass L1_5Term.
-Definition L1_5Env := environ L1_5Term.
+Definition L1gTerm := L1g.compile.Term.
+Definition L1gTerms := L1g.compile.Terms.
+Definition L1gDefs := L1g.compile.Defs.
+Definition L1gPgm := Program L1gTerm.
+Definition L1gEC := envClass L1gTerm.
+Definition L1gEnv := environ L1gTerm.
 
 
 Inductive Term : Type :=
 | TRel       : nat -> Term
 | TSort      : Srt -> Term
-| TProof     : Term
+| TProof     : Term -> Term
 | TCast      : Term -> Term
 | TProd      : name -> Term -> Term
 | TLambda    : name -> Term -> Term
@@ -36,7 +37,7 @@ Inductive Term : Type :=
 | TAx        : Term
 | TInd       : inductive -> Term
 | TConstruct : inductive -> nat (* cnstr no *) -> nat (* arity *) -> Term
-| TCase      : (inductive * nat * list nat) (* # parameters, # args per branch *) ->
+| TCase      : (inductive * nat * list nat) (* # params, args per branch *) ->
                Term -> Terms -> Term
 | TFix       : Defs -> nat -> Term
 | TWrong     : Term
@@ -58,55 +59,65 @@ Notation type_ := (TSort SType).
 Notation tunit t := (tcons t tnil).
 
 
-Function strip (t:L1_5Term) : Term :=
+Function strip (t:L1gTerm) : Term :=
   match t with
-    | L1_5.compile.TProof => TProof
-    | L1_5.compile.TRel n => TRel n
-    | L1_5.compile.TSort s => TSort s
-    | L1_5.compile.TCast t _ _ => TCast (strip t)
-    | L1_5.compile.TProd nm _ bod => TProd nm (strip bod)
-    | L1_5.compile.TLambda nm _ bod => TLambda nm (strip bod)
-    | L1_5.compile.TLetIn nm dfn _ bod =>
+    | L1g.compile.TRel n => TRel n
+    | L1g.compile.TSort s => TSort s
+    | L1g.compile.TCast t _ (L1g.compile.TCast _ _ (L1g.compile.prop)) =>
+      TProof (strip t)
+    | L1g.compile.TCast t _ _ => TCast (strip t)
+    | L1g.compile.TProd nm _ bod => TProd nm (strip bod)
+    | L1g.compile.TLambda nm _ bod => TLambda nm (strip bod)
+    | L1g.compile.TLetIn nm dfn _ bod =>
       TLetIn nm (strip dfn) (strip bod)
-    | L1_5.compile.TApp fn arg args =>
+    | L1g.compile.TApp fn arg args =>
       TApp (strip fn) (strip arg) (strips args)
-    | L1_5.compile.TConst nm => TConst nm
-    | L1_5.compile.TAx => TAx
-    | L1_5.compile.TInd i => TInd i
-    | L1_5.compile.TConstruct i m arty => TConstruct i m arty
-    | L1_5.compile.TCase n _ mch brs => TCase n (strip mch) (strips brs)
-    | L1_5.compile.TFix ds n => TFix (stripDs ds) n
-    | L1_5.compile.TWrong => TWrong
+    | L1g.compile.TConst nm => TConst nm
+    | L1g.compile.TAx => TAx
+    | L1g.compile.TInd i => TInd i
+    | L1g.compile.TConstruct i m arty => TConstruct i m arty
+    | L1g.compile.TCase n _ mch brs => TCase n (strip mch) (strips brs)
+    | L1g.compile.TFix ds n => TFix (stripDs ds) n
+    | L1g.compile.TWrong _ => TWrong
   end
-with strips (ts:L1_5Terms) : Terms := 
+with strips (ts:L1gTerms) : Terms := 
   match ts with
-    | L1_5.compile.tnil => tnil
-    | L1_5.compile.tcons t ts => tcons (strip t) (strips ts)
+    | L1g.compile.tnil => tnil
+    | L1g.compile.tcons t ts => tcons (strip t) (strips ts)
   end
-with stripDs (ts:L1_5Defs) : Defs := 
+with stripDs (ts:L1gDefs) : Defs := 
   match ts with
-    | L1_5.compile.dnil => dnil
-    | L1_5.compile.dcons nm _ t m ds => dcons nm (strip t) m (stripDs ds)
+    | L1g.compile.dnil => dnil
+    | L1g.compile.dcons nm _ t m ds => dcons nm (strip t) m (stripDs ds)
   end.
 
+Lemma notPrf_stripCast:
+  forall x, ~ L1g.term.isProp x ->
+  forall t1 ck1 t2 ck2,
+    strip (L1g.compile.TCast
+             t1 ck1 (L1g.compile.TCast t2 ck2 x)) = TCast (strip t1).
+  destruct x; intros; cbn; try reflexivity.
+  destruct s; try reflexivity.
+  elim H. reflexivity.
+Qed.
 
 (** environments and programs **)
-Function stripEC (ec:L1_5EC) : AstCommon.envClass Term :=
+Function stripEC (ec:L1gEC) : AstCommon.envClass Term :=
   match ec with
     | ecTrm t => ecTrm (strip t)
     | ecTyp _ n itp => ecTyp Term n itp
   end.
 
-Definition  stripEnv : L1_5Env -> AstCommon.environ Term :=
-  List.map (fun nmec : string * L1_5EC => (fst nmec, stripEC (snd nmec))).
+Definition  stripEnv : L1gEnv -> AstCommon.environ Term :=
+  List.map (fun nmec : string * L1gEC => (fst nmec, stripEC (snd nmec))).
 
-Definition stripProgram (p:L1_5Pgm) : Program Term :=
+Definition stripProgram (p:L1gPgm) : Program Term :=
   {| env:= stripEnv (env p);
      main:= strip (main p) |}.
 
 (*** from L1 to L2 ***) 
 Definition program_Program (p:program) : Program Term :=
-  stripProgram (L1_5.compile.program_Program p).
+  stripProgram (L1g.compile.program_Program p).
 
 Definition term_Term (e:AstCommon.environ L1gTerm) (t:term) : Term :=
-  strip (L1_5.compile.term_Term e t).
+  strip (L1g.compile.term_Term e t).
