theories/L2_typeStripped/stripWndCommute.v
@@ -1,6 +1,6 @@
 (******)
 Add LoadPath "../common" as Common.
-Add LoadPath "../L1_5_box" as L1_5.
+Add LoadPath "../L1g_box" as L1g.
 Add LoadPath "../L2_typeStripped" as L2.
 (******)
 
@@ -12,25 +12,23 @@ Require Import Coq.Arith.Peano_dec.
 Require Import Coq.Setoids.Setoid.
 Require Import Omega.
 
-Require Import L1_5.L1_5.
+Require Import L1g.L1g.
 Require Import L2.program.
 Require Import L2.wndEval.
 Require Import L2.stripEvalCommute.
 Require Import L2.term.
 Require Import L2.compile.
 
-Definition L1_5Term := L1_5.compile.Term.
-Definition L1_5Terms := L1_5.compile.Terms.
-Definition L1_5Defs := L1_5.compile.Defs.
+Definition L1gTerm := L1g.compile.Term.
+Definition L1gTerms := L1g.compile.Terms.
+Definition L1gDefs := L1g.compile.Defs.
 
 
 Lemma not_isApp_strip_hom:
-  forall (t:L1_5Term), ~ L1_5.term.isApp t -> ~ isApp (strip t).
+  forall (t:L1gTerm), ~ L1g.term.isApp t -> ~ isApp (strip t).
 Proof.
-  destruct t; cbn; intros; try not_isApp.
-  elim H. unfold L1_5.term.isApp. exists t1, t2, t3. reflexivity.
+  intros. intros h. destruct H. apply isApp_hom. assumption.
 Qed.
-
 
 Lemma TApp_mkApp_step_lem:
   forall fn fn' arg args,
@@ -50,28 +48,27 @@ Proof.
   elim H. exists fn1, fn2, t. reflexivity.
 Qed.
 
-(** Since L1_5.wndEval.wndEval may make steps in parts of a term that are
+(** Since L1g.wndEval.wndEval may make steps in parts of a term that are
 *** erased in L2, and since L2.WndEval is not reflexive, we add <>
 ***  hypotheses.
 **)
 Lemma Wnd_hom:
-  forall p, L1_5.program.WFaEnv p ->
-  (forall (s t:L1_5Term),
-     L1_5.wndEval.wndEval p s t ->
-     L1_5.term.WFapp s -> strip s <> strip t ->
+  forall p, L1g.program.WFaEnv p ->
+  (forall (s t:L1gTerm),
+     L1g.wndEval.wndEval p s t ->
+     L1g.term.WFapp s -> strip s <> strip t ->
      wndEval (stripEnv p) (strip s) (strip t)) /\
-  (forall (ss ts:L1_5Terms),
-     L1_5.wndEval.wndEvals p ss ts ->
-     L1_5.term.WFapps ss -> strips ss <> strips ts ->
+  (forall (ss ts:L1gTerms),
+     L1g.wndEval.wndEvals p ss ts ->
+     L1g.term.WFapps ss -> strips ss <> strips ts ->
      wndEvals (stripEnv p) (strips ss) (strips ts)).
 Proof.
   intros p hp.
-  apply L1_5.wndEval.wndEvalEvals_ind; intros; try (solve [constructor]);
+  apply L1g.wndEval.wndEvalEvals_ind; intros; try (solve [constructor]);
   try (solve[cbn in H1; elim H1; reflexivity]);
   try (solve[cbn in H1; constructor; apply H; [
     inversion_Clear H0; assumption |
-    intros h; elim H1; rewrite h; reflexivity]]);
-  cbn.
+    intros h; elim H1; rewrite h; reflexivity]]).
   - constructor.
     + apply LookupDfn_hom. assumption.
   - rewrite whBetaStep_hom. constructor.
@@ -84,6 +81,7 @@ Proof.
     refine (sFix _ _ _ _ _ _).
     rewrite <- dnthBody_hom. rewrite <- optStripDnth_hom.
     apply f_equal. eassumption.
+  - admit.
   - rewrite mkApp_hom. refine (sAppFn _ _ _). inversion_Clear H0.
     apply H. assumption.
     + rewrite TApp_hom in H1. rewrite mkApp_hom in H1.
@@ -97,33 +95,35 @@ Proof.
     inversion_Clear H0. apply H.
     + constructor; assumption.
     + intros h. myInjection h. elim H1. rewrite H0, H2. reflexivity.
-Qed.
+Admitted.
 
 Lemma TConst_strip_inv:
-  forall nm r, TConst nm = strip r -> r = L1_5.compile.TConst nm.
+  forall nm r, TConst nm = strip r -> r = L1g.compile.TConst nm.
 Proof.
-  destruct r; cbn; intros; try discriminate. myInjection H. reflexivity.
-Qed.
+  destruct r; intros; try discriminate.
+  - admit.
+  - myInjection H. reflexivity.
+Admitted.
 
 
 (**************************
-Lemma L2wnd_L1_5wnd:
+Lemma L2wnd_L1gwnd:
   forall (p:environ),
   (forall (s t:Term), wndEval p s t ->
      forall pp, p = stripEnv pp ->
      forall ss, s = strip ss ->
      forall tt, t = strip tt ->
-     L1_5.wndEval.wndEval pp ss tt) /\
+     L1g.wndEval.wndEval pp ss tt) /\
   (forall (s t:Terms), wndEvals p s t ->
      forall pp, p = stripEnv pp ->
      forall ss, s = strips ss ->
      forall tt, t = strips tt ->
-     L1_5.wndEval.wndEvals pp ss tt) /\
+     L1g.wndEval.wndEvals pp ss tt) /\
   (forall (s t:Defs), wndDEvals p s t ->
      forall pp, p = stripEnv pp ->
      forall ss, s = stripDs ss ->
      forall tt, t = stripDs tt ->
-     L1_5.wndEval.wndDEvals pp ss tt).
+     L1g.wndEval.wndDEvals pp ss tt).
 Proof.
   intros p.
   apply wndEvalEvals_ind; intros; subst.
